test/FiniteSetEvaluatorFixtures.lean
@@ -4,24 +4,16 @@ import EventB.POGSoundness
 
 namespace EventB.POG
 
-private
-def setEnv
-    : ValueEnv :=
+private def setEnv : ValueEnv :=
   { values := [("S", .set [.integer 0, .integer 1])] }
 
-private
-def badSetEnv
-    : ValueEnv :=
+private def badSetEnv : ValueEnv :=
   { values := [("S", .set [.integer 0, .boolean true])] }
 
-private
-def integerUniverseEnv
-    : ValueEnv :=
+private def integerUniverseEnv : ValueEnv :=
   { values := [("S", .integerSet)] }
 
-private
-def setTransition
-    : CheckedBeforeAfter :=
+private def setTransition : CheckedBeforeAfter :=
   { before := setEnv
     after := { values := [("S", .set [.integer 1])] }
     declarations := [("S", .pow .int)] }
@@ -45,9 +37,7 @@ def setTransition
   | .error _ => true
   | .ok _ => false
 
-private
-def witnessBody
-    : EventB.Formula.Term :=
+private def witnessBody : EventB.Formula.Term :=
   .bin "=" (.id "p") (.num 0)
 
 #guard evalPredicateOverFiniteDomain 128 {} "p"
