test/GuardFixtures.lean
@@ -4,9 +4,7 @@ import EventB.POG.RefinementAdapters
 
 namespace EventB.POG
 
-private
-def guardedProject
-    : EventB.Typing.Project :=
+private def guardedProject : EventB.Typing.Project :=
   [{ name := "M"
      elem := .machineFile [("org.eventb.core.name", "M")]
        [.variable [("org.eventb.core.identifier", "x")] []
@@ -17,9 +15,7 @@ def guardedProject
           [.guard [("org.eventb.core.label", "g"),
                    ("org.eventb.core.predicate", "x ∈ ℤ")] []]] }]
 
-private
-def malformedGuardProject
-    : EventB.Typing.Project :=
+private def malformedGuardProject : EventB.Typing.Project :=
   [{ name := "M"
      elem := .machineFile [("org.eventb.core.name", "M")]
        [.event [("org.eventb.core.label", "step")]
